mont_mul_add seems to work

lib/bv32_mm_lemmas.i.dfy
@@ -4,8 +4,13 @@ include "bv32_ops.dfy"
 
 module bv32_mm_lemmas refines generic_mm_lemmas {
     import opened GBV = bv32_ops
+    import opened rv_machine
 
     type uint64_view_t = dw_view_t
+
+    const NA : int := -1;
+
+    const NUM_WORDS := 96;
 
     predicate valid_uint64_view(
         num: uint64_view_t,
@@ -27,6 +32,54 @@ module bv32_mm_lemmas refines generic_mm_lemmas {
         dw_split_lemma(full);
 
         GBV.BVSEQ.LemmaSeqLen2([c, d]);
+    }
+
+    datatype mma_vars = mma_vars(
+        frame_ptr: uint32, // writable
+        iter_a: iter_t,
+        a_i: uint32,
+        i: nat,
+        // d0: uint32,
+        iter_b: iter_t,
+        iter_c: iter_t, // writable
+        iter_n: iter_t
+    )
+
+    predicate mvar_iter_inv(mem: mem_t, iter: iter_t, address: int, index: int, value: int)
+    {
+        && (address >= 0 ==> iter_inv(iter, mem, address))
+        && (value >= 0 ==> to_nat(iter.buff) == value)
+        && (index >= 0 ==> iter.index == index)
+        && |iter.buff| == NUM_WORDS
+    }
+
+    predicate mma_vars_inv(
+        vars: mma_vars,
+        mem: mem_t,
+        n_ptr: int, n_idx: int,
+        c_ptr: int, c_idx: int,
+        b_ptr: int, b_idx: int,
+        rsa: rsa_params)
+    {
+        && valid_frame_ptr(mem, vars.frame_ptr, 12)
+
+        && mvar_iter_inv(mem, vars.iter_a, -1, vars.i, NA)
+        && vars.i <= NUM_WORDS
+        && (vars.i < NUM_WORDS ==> vars.iter_a.buff[vars.i] == vars.a_i)
+        && mvar_iter_inv(mem, vars.iter_n, n_ptr, n_idx, rsa.M)
+        && mvar_iter_inv(mem, vars.iter_c, c_ptr, c_idx, NA)
+        && mvar_iter_inv(mem, vars.iter_b, b_ptr, b_idx, NA)
+
+        && vars.iter_c.base_addr != vars.iter_a.base_addr
+        && vars.iter_c.base_addr != vars.iter_n.base_addr
+        && vars.iter_c.base_addr != vars.iter_b.base_addr
+        && vars.iter_c.base_addr != vars.frame_ptr
+
+        && vars.frame_ptr != vars.iter_a.base_addr
+        && vars.frame_ptr != vars.iter_n.base_addr
+        && vars.frame_ptr != vars.iter_b.base_addr
+
+        && rsa_params_inv(rsa)
     }
 
 
