impl/riscv/sub_mod_nl_lemmas.i.dfy
@@ -1,5 +1,3 @@
-include "rsa_ops.i.dfy"
-
 module sub_mod_nl_lemmas {
     import opened bv_ops
     import opened rv_machine
